Removed sorry from HOTG_Cardinals_Base

HOTG/Cardinals/HOTG_Cardinals_Base.thy
@@ -6,9 +6,12 @@ theory HOTG_Cardinals_Base
     Transport.Binary_Relations_Least
     HOTG_Equipollence
     HOTG_Ordinals_Base
+    HOTG_Less_Than
+    HOTG_Choice
 begin
 
 unbundle no_HOL_groups_syntax
+unbundle no_HOL_order_syntax
 
 paragraph \<open>Summary\<close>
 text \<open>Translation of cardinality from HOL-Library and \<^cite>\<open>ZFC_in_HOL_AFP\<close>.
@@ -17,15 +20,16 @@ The cardinality of a set \<open>X\<close> is the smallest ordinal number \<open>
 exists a bijection between \<open>X\<close> and \<open>\<alpha>\<close>.
 Further details can be found in \<^url>\<open>https://en.wikipedia.org/wiki/Cardinal_number\<close>.\<close>
 
-definition "cardinality (X :: set) \<equiv> least_wrt_rel (\<subseteq>) (ordinal \<sqinter> ((\<approx>) X))"
+(* Verwende (\<le>) statt (\<subseteq>) da (\<le>)/(\<subseteq>) auf Ordinalzahlen äquivalent sind und (\<le>) hier bequemer ist. *)
+definition "cardinality (X :: set) \<equiv> least_wrt_rel (\<le>) (ordinal \<sqinter> ((\<approx>) X))"
 
 bundle hotg_cardinality_syntax begin notation cardinality ("|_|") end
 bundle no_hotg_cardinality_syntax begin no_notation cardinality ("|_|") end
 unbundle hotg_cardinality_syntax
 
-lemma cardinality_eq_if_equipollent_if_subset_if_ordinal:
+lemma cardinality_eq_if_equipollent_if_le_if_ordinal:
   assumes "ordinal Y"
-  and "\<And>Y'. ordinal Y' \<Longrightarrow> X \<approx> Y' \<Longrightarrow> Y \<subseteq> Y'"
+  and "\<And>Y'. ordinal Y' \<Longrightarrow> X \<approx> Y' \<Longrightarrow> Y \<le> Y'"
   and "X \<approx> Y"
   shows "|X| = Y"
   unfolding cardinality_def using assms by (intro least_wrt_rel_eq_if_antisymmetric_onI) auto
@@ -40,13 +44,41 @@ text\<open>The next lemma shows that \<open>X\<close> is equipollent with @{term
 The proof requires order types, which are currently missing.  For a proof, see
 \<^url>\<open>https://foss.heptapod.net/isa-afp/afp-devel/-/blob/06458dfa40c7b4aaaeb855a37ae77993cb4c8c18/thys/ZFC_in_HOL/ZFC_Cardinals.thy#L1829\<close>.\<close>
 
-lemma cardinality_equipollent_self [iff]: "|X| \<approx> X"
-  sorry
+lemma least_ordinal_with_prop_welldefined_if_witness:
+  assumes "P \<gamma>" and ordinal_if_P: "\<forall>\<alpha> : P. ordinal \<alpha>"
+  shows "is_least_wrt_rel (\<le>) P (least_wrt_rel (\<le>) P)"
+proof -
+  from \<open>P \<gamma>\<close> obtain \<alpha> where "P \<alpha>" and \<alpha>_minimal: "\<And>\<beta>. \<beta> < \<alpha> \<Longrightarrow> \<not> P \<beta>" 
+    using lt_minimal_set_witnessE by blast
+  have \<alpha>_least: "\<alpha> \<le> \<beta>" if "P \<beta>" for \<beta>
+  proof -
+    have "ordinal \<alpha>" "ordinal \<beta>" using \<open>P \<alpha>\<close> \<open>P \<beta>\<close> ordinal_if_P by auto
+    then show ?thesis using that \<alpha>_minimal by (cases rule: lt_eq_lt_if_ordinalE) auto
+  qed
+  then have "is_least_wrt_rel (\<le>) P \<alpha>" 
+    using \<open>P \<alpha>\<close> by (auto intro!: is_least_wrt_rel_if_antisymmetric_onI)
+  then show ?thesis using least_wrt_rel_eqI by force
+qed
+
+lemma
+  ordinal_cardinality: "ordinal |X|" and
+  cardinality_equipollent_self [iff]: "|X| \<approx> X" and
+  cardinality_le_if_equipollent_ordinal: "\<forall>\<beta> : ordinal. X \<approx> \<beta> \<longrightarrow> |X| \<le> \<beta>"
+proof -
+  define P where "P \<equiv> ordinal \<sqinter> ((\<approx>) X)"
+  from equipollent_some_ordinal obtain \<alpha> where "ordinal \<alpha>" "X \<approx> \<alpha>" by blast
+  then have "P \<alpha>" "\<forall>\<beta> : P. ordinal \<beta>" using P_def by auto
+  then have least: "is_least_wrt_rel (\<le>) P |X|" 
+    using cardinality_def P_def least_ordinal_with_prop_welldefined_if_witness by auto
+  then show "ordinal |X|" "|X| \<approx> X" "\<forall>\<beta> : ordinal. X \<approx> \<beta> \<longrightarrow> |X| \<le> \<beta>" 
+    using P_def symmetric_equipollent 
+    by (auto elim!: is_least_wrt_relE is_minimal_wrt_relE dest: symmetricD)
+qed
 
 lemma cardinality_cardinality_eq_cardinality [simp]: "||X|| = |X|"
   by (intro cardinality_eq_if_equipollent cardinality_equipollent_self)
 
 lemma cardinality_zero_eq_zero [simp]: "|0| = 0"
-  by (intro cardinality_eq_if_equipollent_if_subset_if_ordinal) auto
+  by (intro cardinality_eq_if_equipollent_if_le_if_ordinal) (auto simp: zero_le_if_ordinal)
 
 end
